@prefix dc: <http://purl.org/dc/elements/1.1/> .
@prefix dcterms: <http://purl.org/dc/terms/> .
@prefix skos: <http://www.w3.org/2004/02/skos/core#> .
@prefix xml: <http://www.w3.org/XML/1998/namespace> .
@prefix xsd: <http://www.w3.org/2001/XMLSchema#> .
@prefix vs: <http://www.w3.org/2003/06/sw-vocab-status/ns#> .
@prefix adms: <http://www.w3.org/ns/adms#> .
@prefix resourceType: <http://purl.org/dcx/lrmi-vocabs/learningResourceType/> .
@prefix bibo: <http://purl.org/ontology/bibo/status/> .
@prefix loc: <http://id.loc.gov/authorities/genreForms/> .

resourceType: a skos:ConceptScheme ;
    dc:title "LRMI Learning Resource Type Concept Scheme"@en-US ;
    dc:creator "LRMI Task Group (DCMI)"@en-US ;
    dcterms:dateSubmitted "2022-01-25"^^xsd:date ;
    dc:description "A concept scheme that enumerates different types of learning resource. By learning resource we mean a persistent resource that has one or more physical or digital representation, and that explicitly involves, specifies or entails a learning activity or learning experience."@en-US ;
    dc:source <https://ceds.ed.gov/element/000928> ;
    adms:status bibo:published .

resourceType:actvityPlan a skos:Concept ;
    skos:prefLabel "activity plan"@en-US ;
    skos:definition "Detailed description of an activity engaged in by the learner for the purpose of acquiring certain skills, concepts, or knowledge, whether guided by an instructor or not."@en-US ;
    skos:scopeNote "There may be several activities in a lesson or an activity may take place outside of a lesson." ;
    skos:inScheme resourceType: ;
    skos:relatedMatch loc:gf2018026088 ;  #Lesson plans
    skos:exactMatch <https://ceds.ed.gov/element/000928#LearningActivity> ;
    dcterms:source <https://ceds.ed.gov/element/000928#LearningActivity> ;
    vs:term_status "stable" .

resourceType:assessment a skos:Concept ;
    skos:prefLabel "assessment"@en-US ;
    skos:definition "Set of assessment items used to evaluate or promote learning."@en-US ;
    skos:inScheme resourceType: ;
    skos:closeMatch loc:gf2014026096 ; #Examinations
    skos:relatedMatch loc:gf2014026154 ; # Problems and exercises
    skos:narrowMatch <https://ceds.ed.gov/element/000928#AlternateAssessment> ,
         <https://ceds.ed.gov/element/000928#FormativeAssessment> ,
         <https://ceds.ed.gov/element/000928#InterimSummativeAssessment> ,
         <https://ceds.ed.gov/element/000928#SelfAssessment> ;
    vs:term_status "stable" .

resourceType:assessmentItem a skos:Concept ;
    skos:prefLabel "assessment item"@en-US ;
    skos:definition "Specific prompt, that defines a question or protocol for a measurable activity that triggers a response from a person used to determine whether the person has mastered a learning objective."@en-US ;
    skos:inScheme resourceType: ;
    skos:broadMatch loc:gf2014026096 ; #Examinations
    skos:narrowMatch loc:gf2014026154 ; # Problems and exercises
    skos:exactMatch <https://ceds.ed.gov/element/000928#AssessmentItem> ;
    dcterms:source <https://ceds.ed.gov/element/000928#AssessmentItem> ;
    vs:term_status "stable" .

resourceType:educatorCurriculumGuide a skos:Concept ;
    skos:prefLabel "educator curriculum guide"@en-US ;
    skos:definition "Document that defines what concepts should be taught and/or how a concept should be taught effectively."@en-US ;
    skos:inScheme resourceType: ;
    skos:broadMatch loc:gf2014026188 ; # Teachers' guides
    skos:exactMatch <https://ceds.ed.gov/element/000928#EducatorCurriculumGuide> ;
    dcterms:source <https://ceds.ed.gov/element/000928#EducatorCurriculumGuide> ;
    vs:term_status "stable" .

resourceType:lessonPlan a skos:Concept ;
    skos:prefLabel "lesson plan"@en-US ;
    skos:definition "Detailed description of the course of instruction for a Â­short period of time that is used by a teacher to guide class instruction."@en-US ;
    skos:usageNote "Several lessons on the same topic would be a Unit. A lesson may include one or more learning activities." ;
    skos:inScheme resourceType: ;
    skos:exactMatch loc:gf2018026088 ; # Lesson Plans
    skos:exactMatch <https://ceds.ed.gov/element/000928#Lesson> ;
    dcterms:source <https://ceds.ed.gov/element/000928#Lesson> ;
    vs:term_status "stable" .

resourceType:physicalLearningResource a skos:Concept ;
    skos:prefLabel "physical learning resource"@en-US ;
    skos:definition "Physical object, hardware or device designed to help a learner achieve some learning objective."@en-US ;
    skos:scopeNote "Examples include educational toys, programmable robots, manipulables used by learners. This does not include auxiliary resources (e.g. pencil, paper, scissors, soldering iron) required for a learning activity." ;
    skos:inScheme resourceType: ;
    skos:narrowMatch loc:gf2018026057 ; # Manipulatives
    vs:term_status "stable" .

resourceType:recordedLesson a skos:Concept ;
    skos:prefLabel "recorded lesson"@en-US ;
    skos:definition "Audio or video recording, or textual record (e.g. transcript or edited script) of a lesson, lecture or similar short instructional event."@en-US ;
    skos:inScheme resourceType: ;
    skos:relatedMatch loc:gf2011026219 ; # Educational films
    skos:relatedMatch loc:gf2014026122 ; # Lectures
    vs:term_status "stable" .

resourceType:supportingDocument a skos:Concept ;
    skos:prefLabel "supporting document"@en-US ;
    skos:definition "Document with an instructional component designed to help a learner achieve some learning objective."@en-US ;
    skos:scopeNote "These are typically static text and or images that may be physical or online. Examples include training manuals, infographics, explainers, textbook chapters, slides from a lesson in whatever form. For textbooks use Textbook. This does not include supplementary/auxilliary resources (e.g. the text being studied in a language class) required for a learning activity." ;
    skos:inScheme resourceType: ;
    skos:narrowMatch loc:gf2014026073 ; # Course materials
    dcterms:source <http://oerschema.org/SupportingMaterial/> ;
    vs:term_status "stable" .

resourceType:textbook a skos:Concept ;
    skos:prefLabel "textbook"@en-US ;
    skos:definition "Book designed to be used as a standard source of information to facilitate learning of  a particular subject."@en-US ;
    skos:inScheme resourceType: ;
    skos:exactMatch loc:gf2014026191 ; # Textbooks
    skos:exactMatch <https://ceds.ed.gov/element/000928#Textbook> ;
    dcterms:source <https://ceds.ed.gov/element/000928#Textbook> ;
    vs:term_status "stable" .

resourceType:unitPlan a skos:Concept ;
    skos:prefLabel "unit plan"@en-US ;
    skos:definition "Long-range plan of instruction on a particular concept. "@en-US ;
    skos:scopeNote "A Unit contains several lessons, activities and or assessments that are related."@en-US ;
    skos:inScheme resourceType: ;
    skos:broadMatch loc:gf2014026114 ;# Instructional and educational works
    skos:exactMatch <https://ceds.ed.gov/element/000928#Unit> ;
    dcterms:source <https://ceds.ed.gov/element/000928#Unit> ;
    vs:term_status "stable" .
