@prefix lrmi: <http://purl.org/dcx/lrmi-terms/> .
@prefix dcterms: <http://purl.org/dc/terms/> .
@prefix owl: <http://www.w3.org/2002/07/owl#> .
@prefix rdf: <http://www.w3.org/1999/02/22-rdf-syntax-ns#> .
@prefix rdfs: <http://www.w3.org/2000/01/rdf-schema#> .
@prefix schema: <http://schema.org/> .
@prefix xml: <http://www.w3.org/XML/1998/namespace> .
@prefix xsd: <http://www.w3.org/2001/XMLSchema#> .
@prefix vann: <http://purl.org/vocab/vann/> .

# SCHEMA DESCRIPTION

<http://purl.org/dcx/lrmi-terms/> dcterms:creator "LRMI Task Group"@en ;
    dcterms:description "The LRMI specification is a collection of classes and properties for markup and description of educational resources. The specification builds on the extensive vocabulary provided by Schema.org and other standards. Note: the labels provided here are not considered normative."@en ;
    dcterms:identifier <http://dublincore.org/dcx/lrmi-terms/> ;
    dcterms:isVersionOf <http://purl.org/dcx/lrmi-terms/1.1/> ;
    dcterms:issued "2015-02-09"^^xsd:date ;
    dcterms:license <https://creativecommons.org/licenses/by/4.0/> ;
    dcterms:title "LRMI RDF Specification"@en .

# CLASSES
lrmi:AlignmentObject a rdfs:Class ;
    rdfs:label "Alignment Object"@en ;
    dcterms:issued "2015-02-09"^^xsd:date ;
    rdfs:comment "An intangible item that describes an alignment between a learning resource and a node in an educational framework."@en ;
    rdfs:subClassOf schema:Intangible ;
    owl:equivalentClass schema:AlignmentObject ;
    rdfs:isDefinedBy <http://purl.org/dcx/lrmi-terms/> .

lrmi:EducationalAudience a rdfs:Class ;
    rdfs:label "Educational Audience"@en ;
    dcterms:issued "2015-02-09"^^xsd:date ;
    rdfs:comment "An individual or group for whom the learning resource was created or useful."@en ;
    rdfs:subClassOf schema:Intangible ;
    owl:equivalentClass schema:EducationalAudience ;
    rdfs:isDefinedBy <http://purl.org/dcx/lrmi-terms/> .

lrmi:LearningResource a rdfs:Class ;
    rdfs:label "Learning Resource"@en ;
    dcterms:issued "2020-08-31"^^xsd:date ;
    rdfs:comment "A persistent resource that has one or more physical or digital representations, and that explicitly involves, specifies or entails a learning activity or learning experience."@en ;
    skos:scopeNote "The LearningResource type can be used to indicate creative works (whether physical or digital) that have a particular and explicit orientation towards learning, education, training, skill acquisition, and other learning purposes. LearningResource is expected to be used as an addition to a primary type such as http://purl.org/ontology/bibo/Book, https://schema.org/Video, http://purl.org/dc/terms/PhysicalResource etc."@en ;
    rdfs:subClassOf schema:CreativeWork ;
    owl:equivalentClass schema:LearningResource ;
    rdfs:isDefinedBy <http://purl.org/dcx/lrmi-terms/> .

# PROPERTIES

lrmi:alignmentType a rdf:Property ;
    rdfs:label "Alignment Type"@en ;
    rdfs:comment "A category of alignment between the learning resource and the framework node."@en ;
    skos:scopeNote "Recommended values include: 'assesses', 'teaches', 'requires', 'textComplexity', 'readingLevel', 'educationalSubject', and 'educationLevel'."@en ;
    dcterms:issued "2015-02-09"^^xsd:date ;
    schema:domainIncludes lrmi:AlignmentObject, schema:AlignmentObject ;
    schema:rangeIncludes xsd:string ;
    owl:equivalentProperty schema:alignmentType ;
    rdfs:isDefinedBy <http://purl.org/dcx/lrmi-terms/> .

lrmi:assesses a rdf:Property ;
    rdfs:label "Assesses"@en ;
    rdfs:comment "The item being described is intended to assess the competency or learning outcome defined by the referenced term."@en ;
    dcterms:issued "2020-08-31"^^xsd:date ;
    schema:domainIncludes schema:CreativeWork, lrmi:LearningResource, schema:LearningResource ;
    schema:rangeIncludes schema:DefinedTerm ;
    owl:equivalentProperty schema:assesses ;
    rdfs:isDefinedBy <http://purl.org/dcx/lrmi-terms/> .

lrmi:educationalAlignment a rdf:Property ;
    rdfs:label "Educational Alignment"@en ;
    rdfs:comment "An alignment to an established educational framework."@en ;
    dcterms:issued "2015-02-09"^^xsd:date ;
    schema:domainIncludes schema:CreativeWork, lrmi:LearningResource, schema:LearningResource ;
    schema:rangeIncludes lrmi:AlignmentObject, schema:AlignmentObject ;
    owl:equivalentProperty schema:educationalAlignment ;
    rdfs:isDefinedBy <http://purl.org/dcx/lrmi-terms/> .

lrmi:educationalFramework a rdf:Property ;
    rdfs:label "Educational Framework"@en ;
    rdfs:comment "The framework to which the resource being described is aligned."@en ;
    dcterms:issued "2015-02-09"^^xsd:date ;
    schema:domainIncludes lrmi:AlignmentObject, schema:AlignmentObject ;
    schema:rangeIncludes xsd:string ;
    owl:equivalentProperty schema:educationalFramework ;
    rdfs:isDefinedBy <http://purl.org/dcx/lrmi-terms/> .

lrmi:educationalLevel a rdf:Property ;
    rdfs:label "Educational Level"@en ;
    rdfs:comment "The level of a resource in terms of progression through an educational or training context." ;
    skos:scopeNote "Examples of educational levels include 'beginner', 'intermediate' or 'advanced', and formal sets of level indicators."@en ;
    dcterms:issued "2020-08-31"^^xsd:date ;
    schema:domainIncludes schema:CreativeWork, lrmi:LearningResource, schema:LearningResource ;
    schema:rangeIncludes schema:DefinedTerm, xsd:string, xsd:anyURI ;
    owl:equivalentProperty schema:assesses ;
    rdfs:isDefinedBy <http://purl.org/dcx/lrmi-terms/> .

lrmi:educationalRole a rdf:Property ;
    rdfs:label "Educational Role"@en ;
    rdfs:comment "The role that describes the target audience of the content."@en ;
    skos:scopeNote "The educational function assumed or part played by the group for whom the resource is intended."@en ;
    dcterms:issued "2015-02-09"^^xsd:date ;
    schema:domainIncludes lrmi:EducationalAudience, schema:EducationalAudience ;
    schema:rangeIncludes xsd:string ;
    owl:equivalentProperty schema:educationalRole ;
    rdfs:isDefinedBy <http://purl.org/dcx/lrmi-terms/> .

lrmi:educationalUse a rdf:Property ;
    rdfs:label "Educational Use"@en ;
    rdfs:comment "The purpose of a work in the context of education."@en ;
    skos:scopeNote "For example, 'assignment', 'group work'."@en ;
    dcterms:issued "2015-02-09"^^xsd:date ;
    schema:domainIncludes schema:CreativeWork, lrmi:LearningResource, schema:LearningResource ;
    schema:rangeIncludes xsd:string ;
    owl:equivalentProperty schema:educationalUse ;
    rdfs:isDefinedBy <http://purl.org/dcx/lrmi-terms/> .

lrmi:interactivityType a rdf:Property ;
    rdfs:label "Interactivity Type"@en ;
    rdfs:comment "The predominant mode of learning supported by the learning resource."@en ;
    skos:scopeNote "Acceptable values are 'active', 'expositive', or 'mixed'."@en,
        "Based on, and mappable from, IEEE LOM 5.1: Interactivity Type."@en ;
    dcterms:issued "2015-02-09"^^xsd:date ;
    schema:domainIncludes schema:CreativeWork, lrmi:LearningResource, schema:LearningResource ;
    schema:rangeIncludes xsd:string ;
    owl:equivalentProperty schema:interactivityType ;
    rdfs:isDefinedBy <http://purl.org/dcx/lrmi-terms/> .

lrmi:isBasedOnUrl a rdf:Property ;
    rdfs:label "Is Based On"@en ;
    rdfs:comment "A resource from which this work is derived or from which it is a modification or adaption."@en ;
    skos:scopeNote "This term can be repeated for multiple sources."@en ;
    dcterms:issued "2015-02-09"^^xsd:date ;
    schema:domainIncludes schema:CreativeWork ;
    schema:rangeIncludes xsd:anyURI ;
    owl:equivalentProperty schema:isBasedOnUrl, schema:isBasedOn ;
    rdfs:isDefinedBy <http://purl.org/dcx/lrmi-terms/> .

lrmi:learningResourceType a rdf:Property ;
    rdfs:label "Learning Resource Type"@en ;
    rdfs:comment "The predominant type or kind characterizing the learning resource."@en ;
    skos:scopeNote "For example, 'presentation', 'handout'."@en ;
    dcterms:issued "2015-02-09"^^xsd:date ;
    schema:domainIncludes schema:CreativeWork, lrmi:LearningResource, schema:LearningResource ;
    schema:rangeIncludes xsd:string ;
    owl:equivalentProperty schema:learningResourceType ;
    rdfs:isDefinedBy <http://purl.org/dcx/lrmi-terms/> .

lrmi:targetDescription a rdf:Property ;
    rdfs:label "Target Description"@en ;
    rdfs:comment "The description of a node in an established educational framework."@en ;
    dcterms:issued "2015-02-09"^^xsd:date ;
    schema:domainIncludes lrmi:AlignmentObject, schema:AlignmentObject ;
    schema:rangeIncludes xsd:string ;
    owl:equivalentProperty schema:targetDescription ;
    rdfs:isDefinedBy <http://purl.org/dcx/lrmi-terms/> .

lrmi:targetName a rdf:Property ;
    rdfs:label "Target Name"@en ;
    rdfs:comment "The name of a node in an established educational framework."@en ;
    dcterms:issued "2015-02-09"^^xsd:date ;
    schema:domainIncludes lrmi:AlignmentObject, schema:AlignmentObject ;
    schema:rangeIncludes xsd:string ;
    owl:equivalentProperty schema:targetName ;
    rdfs:isDefinedBy <http://purl.org/dcx/lrmi-terms/> .

lrmi:targetUrl a rdf:Property ;
    rdfs:label "Target URL"@en ;
    rdfs:comment "The URL of a node in an established educational framework."@en ;
    dcterms:issued "2015-02-09"^^xsd:date ;
    schema:domainIncludes lrmi:AlignmentObject, schema:AlignmentObject ;
    schema:rangeIncludes xsd:anyURI ;
    owl:equivalentProperty schema:targetUrl ;
    rdfs:isDefinedBy <http://purl.org/dcx/lrmi-terms/> .

lrmi:timeRequired a rdf:Property ;
    rdfs:label "Time Required"@en ;
    rdfs:comment "Approximate or typical time it takes to work with or through this learning resource for the typical intended target audience."@en ;
    skos:scopeNote "Based on, and mappable from, IEEE LOM 5.9: Typical Learning   Time."@en, "For example, 'PT30M' and 'PT1H25M'"@en ;
    dcterms:issued "2015-02-09"^^xsd:date ;
    schema:domainIncludes schema:CreativeWork ;
    schema:rangeIncludes schema:Duration ;
    owl:equivalentProperty schema:timeRequired ;
    rdfs:isDefinedBy <http://purl.org/dcx/lrmi-terms/> .

lrmi:teaches a rdf:Property ;
    rdfs:label "Teaches"@en ;
    rdfs:comment "The item being described is intended to help a person learn the competency or learning outcome defined by the referenced term."@en ;
    dcterms:issued "2020-08-31"^^xsd:date ;
    schema:domainIncludes schema:CreativeWork, lrmi:LearningResource, schema:LearningResource ;
    schema:rangeIncludes schema:DefinedTerm ;
    owl:equivalentProperty schema:teaches ;
    rdfs:isDefinedBy <http://purl.org/dcx/lrmi-terms/> .

lrmi:typicalAgeRange a rdf:Property ;
    rdfs:label "Typical Age Range"@en ;
    rdfs:comment "The typical expected age range."@en ;
    skos:scopeNote "Based on, and mappable from, IEEE LOM 5.7: Typical Age Range."@en, "For example, '7-9', '18-'."@en ;
    dcterms:issued "2015-02-09"^^xsd:date ;
    schema:domainIncludes schema:CreativeWork ;
    schema:rangeIncludes xsd:string ;
    owl:equivalentProperty schema:typicalAgeRange ;
    rdfs:isDefinedBy <http://purl.org/dcx/lrmi-terms/> .

lrmi:useRightsUrl a rdf:Property ;
    rdfs:label "Use Rights URL"@en ;
    rdfs:comment "The URL where the owner specifies permissions for using the   resource."@en ;
    skos:scopeNote """For example: 'http://creativecommons.org/licenses/by/3.0/',
   'http://publisher.com/content-use-description'."""@en ;
    dcterms:issued "2015-02-09"^^xsd:date ;
    schema:domainIncludes schema:CreativeWork ;
    schema:rangeIncludes schema:CreativeWork,
        xsd:anyURI ;
    rdfs:subPropertyOf schema:license ;
    rdfs:isDefinedBy <http://purl.org/dcx/lrmi-terms/> .
